Phi_Semantics/PhiSem_Mem_C_Ag_Ar.thy
@@ -1,0 +1,102 @@
+theory PhiSem_Mem_C_Ag_Ar
+  imports PhiSem_Mem_C PhiSem_Aggregate_Array
+begin
+
+section \<open>Array in Memory\<close>
+
+subsection \<open>Semantics\<close>
+
+debt_axiomatization
+    Map_of_Val_arr: \<open>Map_of_Val (V_array.mk vs) =
+      (\<lambda>path. case path of AgIdx_N i # path' \<Rightarrow>
+                                if i < length vs then Map_of_Val (vs ! i) path' else 1
+                         | _ \<Rightarrow> 1)\<close>
+
+subsection \<open>Syntax\<close>
+
+term \<open>\<m>\<e>\<m>[addr] \<a>\<r>\<r>\<a>\<y>[n] T\<close>
+
+setup \<open>Context.theory_map (
+  Phi_Mem_Parser.add 110 (
+    fn ((ctxt,i), f, Const(\<^const_syntax>\<open>Array\<close>, _) $ n $ T) =>
+        SOME (Const(\<^const_name>\<open>\<phi>Mul_Quant_Tree\<close>, dummyT)
+                $ \<^Const>\<open>AgIdx_N \<^Type>\<open>VAL\<close>\<close>
+                $ (\<^Const>\<open>Len_Intvl \<^Type>\<open>nat\<close>\<close> $ HOLogic.zero $ n)
+                $ f (ctxt,0) T)
+     | X => NONE)
+)\<close>
+
+term \<open>\<m>\<e>\<m>[addr] \<a>\<r>\<r>\<a>\<y>[n] T\<close>
+
+subsection \<open>Reasoning\<close>
+
+subsubsection \<open>ToA Mapper\<close>
+
+text \<open>The following lemma cannot be automated because it is tightly related to the semantics\<close>
+
+lemma split_mem_coerce_array':
+  \<open> \<p>\<r>\<e>\<m>\<i>\<s>\<e> length l = Suc n
+\<Longrightarrow> (l \<Ztypecolon> \<m>\<e>\<m>-\<c>\<o>\<e>\<r>\<c>\<e> \<a>\<r>\<r>\<a>\<y>[Suc n] T) = (take n l \<Ztypecolon> \<m>\<e>\<m>-\<c>\<o>\<e>\<r>\<c>\<e> \<a>\<r>\<r>\<a>\<y>[n] T) * (last l \<Ztypecolon> AG_IDX(n\<^sup>\<t>\<^sup>\<h>) \<^bold>\<rightarrow>\<^sub># \<m>\<e>\<m>-\<c>\<o>\<e>\<r>\<c>\<e> T)\<close>
+  unfolding BI_eq_iff Premise_def
+  apply (clarsimp; rule; clarsimp)
+
+  subgoal for vs
+    apply (rule exI[where x=\<open>to_share \<circ> map_option discrete \<circ> Map_of_Val (V_array.mk (take n vs))\<close>])
+    apply (rule exI[where x=\<open>[AG_IDX(n\<^sup>\<t>\<^sup>\<h>)] \<tribullet>\<^sub>m (to_share \<circ> map_option discrete \<circ> Map_of_Val (last vs))\<close>])
+    apply (auto simp: fun_eq_iff times_fun Map_of_Val_arr push_map_cons_neq sep_disj_fun_def
+                      list_all2_lengthD
+                split: list.split aggregate_index'.split)
+    apply (metis (mono_tags, lifting) comp_apply diff_add_inverse last_conv_nth length_0_conv less_antisym list_all2_lengthD nat.simps(3) plus_1_eq_Suc push_map_cons push_map_mult_nil)
+
+    apply (rule exI[where x=\<open>V_array.mk (take n vs)\<close>],
+        auto simp: fun_eq_iff times_fun Map_of_Val_arr push_map_cons_neq list_all2_lengthD
+             split: list.split aggregate_index'.split)
+    apply (rule exI[where x=\<open>to_share \<circ> map_option discrete \<circ> Map_of_Val (last vs)\<close>],
+        auto simp: fun_eq_iff times_fun Map_of_Val_arr push_map_cons_neq list_all2_lengthD
+             split: list.split aggregate_index'.split,
+        rule exI[where x=\<open>last vs\<close>], clarsimp)
+    by (metis diff_add_inverse last_conv_nth lessI list.size(3) list_all2_conv_all_nth nat.simps(3) plus_1_eq_Suc)
+
+  subgoal for v_h v_t
+    apply (rule exI[where x=\<open>V_array.mk (v_h @ [v_t])\<close>])
+    apply (auto simp: fun_eq_iff times_fun Map_of_Val_arr push_map_cons_neq sep_disj_fun_def
+                      list_all2_lengthD nth_append
+                split: list.split aggregate_index'.split)
+    using less_antisym apply fastforce
+    by (smt (verit, ccfv_SIG) append_eq_conv_conj length_Suc_conv_rev less_antisym list_all2_conv_all_nth nth_append nth_append_length snoc_eq_iff_butlast)
+  .
+
+lemma split_mem_coerce_array:
+  \<open> (\<m>\<e>\<m>-\<c>\<o>\<e>\<r>\<c>\<e> \<a>\<r>\<r>\<a>\<y>[n] T) = \<s>\<l>\<i>\<c>\<e>[0,n] (\<m>\<e>\<m>-\<c>\<o>\<e>\<r>\<c>\<e> T) \<close>
+  apply (induct n,
+      (rule \<phi>Type_eqI_BI; unfold BI_eq_iff; clarsimp; rule;
+       clarsimp simp: Map_of_Val_arr fun_eq_iff atLeast0_lessThan_Suc list_all2_Cons2
+                split: list.split aggregate_index'.split),
+       rule \<phi>Type_eqI_Tr)
+
+  \<medium_left_bracket> for n, l premises Tr
+    split_mem_coerce_array'
+    unfold Tr
+  \<medium_right_bracket> certified by auto_sledgehammer 
+  \<medium_left_bracket> premises Tr 
+    apply_rule split_mem_coerce_array'[symmetric, where n=n and l=x and T=T, unfolded Tr]
+    certified by auto_sledgehammer
+  \<medium_right_bracket>.
+
+lemma [\<phi>reason %\<phi>mapToA_norm]:
+  \<open> \<m>\<a>\<p> g : \<s>\<l>\<i>\<c>\<e>[0,n] (\<m>\<e>\<m>-\<c>\<o>\<e>\<r>\<c>\<e>[sty] U)  \<^emph>[C\<^sub>R] R
+          \<mapsto> \<s>\<l>\<i>\<c>\<e>[0,n] (\<m>\<e>\<m>-\<c>\<o>\<e>\<r>\<c>\<e>[sty] U') \<^emph>[C\<^sub>R] R
+    \<o>\<v>\<e>\<r> f : T \<^emph>[C\<^sub>W] W \<mapsto> T' \<^emph>[C\<^sub>W] W'
+    \<w>\<i>\<t>\<h> \<g>\<e>\<t>\<t>\<e>\<r> getter \<s>\<e>\<t>\<t>\<e>\<r> setter \<i>\<n> D
+
+\<Longrightarrow> \<m>\<a>\<p> g : \<m>\<e>\<m>-\<c>\<o>\<e>\<r>\<c>\<e>[array n sty] (\<a>\<r>\<r>\<a>\<y>[n] U) \<^emph>[C\<^sub>R] R
+          \<mapsto> \<m>\<e>\<m>-\<c>\<o>\<e>\<r>\<c>\<e>[array n sty] (\<a>\<r>\<r>\<a>\<y>[n] U') \<^emph>[C\<^sub>R] R
+    \<o>\<v>\<e>\<r> f : T \<^emph>[C\<^sub>W] W \<mapsto> T' \<^emph>[C\<^sub>W] W'
+    \<w>\<i>\<t>\<h> \<g>\<e>\<t>\<t>\<e>\<r> getter \<s>\<e>\<t>\<t>\<e>\<r> setter \<i>\<n> D \<close>
+  unfolding Guided_Mem_Coercion_def split_mem_coerce_array .
+
+hide_fact split_mem_coerce_array'
+
+
+
+end
